Fix RISC-V modelling by following the spec precisely, adding LUI
hoping that LUI will allow us to get rid of the distinction between
literal bitwidth and register bitwidth (but it will require adding
shift left if wXLEN > wInstr, such as in the 64bit case)

src/Riscv.v
@@ -1,3 +1,4 @@
+Require Import Coq.Lists.List.
 Require Import bbv.Word.
 Require Import compiler.StateMonad.
 Require Import compiler.Decidable.
@@ -5,31 +6,64 @@ Require Import compiler.zcast.
 Require Import compiler.PowerFunc.
 Require Import Coq.omega.Omega.
 
+(* Comments between ``double quotes'' are from quotes from
+   The RISC-V Instruction Set Manual
+   Volume I: User-Level ISA
+   Document Version 2.2
+*)
+
 Section Riscv.
-  Context {wlit: nat}. (* bit width of literals *)
-  Context {wdiff: nat}. (* bit width difference between literals and words *)
-  Notation w := (wlit + wdiff).
-  Context {wjimm: nat}. (* bit width of "jump immediates" *)
-  Context {w_lbound: w >= wjimm}.
-  Context {Reg: Set}. (* register name *)
+
+  (* ``There are 31 general-purpose registers x1-x31, which hold integer values. Register x0 is
+     hardwired to the constant 0. [...] This document uses the term XLEN to refer to the current
+     width of an x register in bits (either 32 or 64).'' *)
+  Variable wXLEN: nat.
+
+  (* Bit width of an instruction, will be 32 *)
+  Variable wInstr: nat.
+
+  (* bit width of most immediates, will equal 12 *)
+  Variable wimm: nat.
+
+  (* bit width of "upper" bits to complete 12-bit immediates, will equal 20 *)
+  Variable wupper: nat.
+
+  Variable w_eq: wimm + wupper = wInstr.
+
+  Variable wimm_nonzero: wimm <> 0.
+
+  Variable wupper_nonzero: wupper <> 0.
+
+  Variable wXLEN_lbound: wXLEN >= wInstr.
+
+  Variable Reg: Set. (* register name *)
+
+  Context {dec_Register: DecidableEq Reg}.
 
   Inductive Register: Set :=
     | RegO: Register
     | RegS: Reg -> Register.
 
   Inductive Instruction: Set :=
-    | Addi(rd: Register)(rs1: Register)(imm12: word wlit): Instruction
+    | Addi(rd: Register)(rs1: Register)(imm12: word wimm): Instruction
+    | Slti(rd: Register)(rs1: Register)(imm12: word wimm): Instruction
+    | Sltiu(rd: Register)(rs1: Register)(imm12: word wimm): Instruction
+    | Lui(rd: Register)(imm20: word wupper): Instruction
     | Add(rd: Register)(rs1: Register)(rs2: Register): Instruction
     | Sub(rd: Register)(rs1: Register)(rs2: Register): Instruction
-    | Mul(rd: Register)(rs1: Register)(rs2: Register): Instruction
-    | Sltu(rd: Register)(rs1: Register)(rs2: Register): Instruction
-    | Sltiu(rd: Register)(rs1: Register)(imm12: word wlit): Instruction
     | And(rd: Register)(rs1: Register)(rs2: Register): Instruction
-    | Beq(rs1: Register)(rs2: Register)(sbimm12: word wlit): Instruction
-    | Bne(rs1: Register)(rs2: Register)(sbimm12: word wlit): Instruction
-    | Blt(rs1: Register)(rs2: Register)(sbimm12: word wlit): Instruction
-    | Bge(rs1: Register)(rs2: Register)(sbimm12: word wlit): Instruction
-    | Jal(rd: Register)(jimm20: word wjimm): Instruction.
+    | Or(rd: Register)(rs1: Register)(rs2: Register): Instruction
+    | Xor(rd: Register)(rs1: Register)(rs2: Register): Instruction
+    | Mul(rd: Register)(rs1: Register)(rs2: Register): Instruction
+    | Slt(rd: Register)(rs1: Register)(rs2: Register): Instruction
+    | Sltu(rd: Register)(rs1: Register)(rs2: Register): Instruction
+    | Beq(rs1: Register)(rs2: Register)(sbimm12: word wimm): Instruction
+    | Bne(rs1: Register)(rs2: Register)(sbimm12: word wimm): Instruction
+    | Blt(rs1: Register)(rs2: Register)(sbimm12: word wimm): Instruction
+    | Bltu(rs1: Register)(rs2: Register)(sbimm12: word wimm): Instruction
+    | Bge(rs1: Register)(rs2: Register)(sbimm12: word wimm): Instruction
+    | Bgeu(rs1: Register)(rs2: Register)(sbimm12: word wimm): Instruction
+    | Jal(rd: Register)(jimm20: word wupper): Instruction.
 
   Definition Seqz(rd: Register)(rs1: Register) := Sltiu rd rs1 $1.
   Definition Snez(rd: Register)(rs1: Register) := Sltu rd RegO rs1.
@@ -37,28 +71,74 @@ Section Riscv.
   Definition InfiniteJal := Jal RegO (wneg $4).
 
   Class RiscvState(M: Type -> Type) := mkRiscvState {
-    getRegister: Register -> M (word w);
-    setRegister: Register -> (word w) -> M unit;
-    loadInst: (word w) -> M Instruction; (* decode already included *)
+    getRegister: Register -> M (word wXLEN);
+    setRegister: Register -> (word wXLEN) -> M unit;
+    loadInst: (word wXLEN) -> M Instruction; (* decode already included *)
     (* not yet:
-    loadWord: (word w) -> M (word w);
-    storeWord: (word w) -> (word w) -> M unit;
+    loadWord: (word wXLEN) -> M (word wXLEN);
+    storeWord: (word wXLEN) -> (word wXLEN) -> M unit;
     *)
-    getPC: M (word w);
-    setPC: word w -> M unit;
+    getPC: M (word wXLEN);
+    setPC: word wXLEN -> M unit;
   }.
 
-  Definition signed_lit_to_word(v: word wlit): word w := nat_cast word eq_refl (sext v wdiff).
+  Definition signed_imm_to_word(v: word wimm): word wXLEN.
+    refine (nat_cast word _ (sext v (wupper + wXLEN - wInstr))). abstract omega.
+  Defined.
 
-  Definition signed_jimm_to_word(v: word wjimm): word w.
-    refine (nat_cast word _ (sext v (w - wjimm))). clear -w_lbound. abstract omega.
+  Definition lossless_double{sz: nat}(v: word sz): word (S sz) := WS false v.
+
+  Definition signed_jimm_to_word(v: word wupper): word wXLEN.
+    refine (nat_cast word _ (sext (lossless_double v) (wXLEN - wupper - 1))). abstract omega.
+  Defined.
+
+  Definition signed_bimm_to_word(v: word wimm): word wXLEN.
+    refine (nat_cast word _ (sext (lossless_double v) (wXLEN - wimm - 1))). abstract omega.
+  Defined.
+
+  (* looks like it's the wrong way round, but that's because the argument order of combine is
+     unintuitive *)
+  Definition lossless_shl{sz: nat}(v: word sz)(n: nat): word (n + sz) := combine (wzero n) v.
+
+  Goal lossless_shl (WO~0~1~1~0~1)%word 4 = (WO~0~1~1~0~1~0~0~0~0)%word. reflexivity. Qed.
+
+  Definition upper_imm_to_word(v: word wupper): word wXLEN.
+    refine (nat_cast word _ (sext (lossless_shl v wimm) (wXLEN - wInstr))). abstract omega.
   Defined.
 
   Definition execute{M: Type -> Type}{MM: Monad M}{RVS: RiscvState M}(i: Instruction): M unit :=
     match i with
+
+    (* ``ADDI adds the sign-extended 12-bit immediate to register rs1. Arithmetic overflow is
+       ignored and the result is simply the low XLEN bits of the result.'' *)
     | Addi rd rs1 imm12 =>
         x <- getRegister rs1;
-        setRegister rd (x ^+ (signed_lit_to_word imm12))
+        setRegister rd (x ^+ (signed_imm_to_word imm12))
+
+    (* ``SLTI (set less than immediate) places the value 1 in register rd if register rs1 is
+       less than the sign-extended immediate when both are treated as signed numbers, else 0 is
+       written to rd.'' *)
+    | Slti rd rs1 imm12 =>
+        x <- getRegister rs1;
+        setRegister rd (if wslt_dec x (signed_imm_to_word imm12) then $1 else $0)
+
+    (* ``SLTIU is similar but compares the values as unsigned numbers (i.e., the immediate is
+       first sign-extended to XLEN bits then treated as an unsigned number).'' *)
+    | Sltiu rd rs1 imm12 =>
+        x <- getRegister rs1;
+        setRegister rd (if wlt_dec x (signed_imm_to_word imm12) then $1 else $0)
+
+    (* RV32I: ``LUI (load upper immediate) is used to build 32-bit constants and uses the U-type
+       format. LUI places the U-immediate value in the top 20 bits of the destination register rd,
+       filling in the lowest 12 bits with zeros.''
+       RV64I: ``LUI (load upper immediate) uses the same opcode as RV32I. LUI places the 20-bit
+       U-immediate into bits 31-12 of register rd and places zero in the lowest 12 bits. The 32-bit
+       result is sign-extended to 64 bits. *)
+    | Lui rd imm20 =>
+        setRegister rd (upper_imm_to_word imm20)
+
+    (* ``ADD and SUB perform addition and subtraction respectively. Overflows are ignored and
+       the low XLEN bits of results are written to the destination. *)
     | Add rd rs1 rs2 =>
         x <- getRegister rs1;
         y <- getRegister rs2;
@@ -67,45 +147,89 @@ Section Riscv.
         x <- getRegister rs1;
         y <- getRegister rs2;
         setRegister rd (x ^- y)
-    | Mul rd rs1 rs2 =>
+
+    (* ``SLT and SLTU perform signed and unsigned compares respectively, writing 1 to rd
+       if rs1 < rs2, 0 otherwise.'' *)
+    | Slt rd rs1 rs2 =>
         x <- getRegister rs1;
         y <- getRegister rs2;
-        setRegister rd (x ^* y)
+        setRegister rd (if wslt_dec x y then $1 else $0)
     | Sltu rd rs1 rs2 =>
         x <- getRegister rs1;
         y <- getRegister rs2;
         setRegister rd (if wlt_dec x y then $1 else $0)
-    | Sltiu rd rs1 imm12 =>
-        x <- getRegister rs1;
-        setRegister rd (if wlt_dec x (signed_lit_to_word imm12) then $1 else $0)
+
+    (* ``AND, OR, and XOR perform bitwise logical operations.'' *)
     | And rd rs1 rs2 =>
         x <- getRegister rs1;
         y <- getRegister rs2;
-        setRegister rd (x ^& y)
-    | Beq rs1 rs2 sbimm12 =>
+        setRegister rd (wand x y)
+    | Or rd rs1 rs2 =>
         x <- getRegister rs1;
         y <- getRegister rs2;
-        pc <- getPC;
-        if weq x y then (setPC (pc ^+ (signed_lit_to_word sbimm12))) else Return tt
-    | Bne rs1 rs2 sbimm12 =>
+        setRegister rd (wor x y)
+    | Xor rd rs1 rs2 =>
         x <- getRegister rs1;
         y <- getRegister rs2;
-        pc <- getPC;
-        if weq x y then Return tt else (setPC (pc ^+ (signed_lit_to_word sbimm12)))
-    | Blt rs1 rs2 sbimm12 =>
-        x <- getRegister rs1;
-        y <- getRegister rs2;
-        pc <- getPC;
-        if wlt_dec x y then (setPC (pc ^+ (signed_lit_to_word sbimm12))) else Return tt
-    | Bge rs1 rs2 sbimm12 =>
-        x <- getRegister rs1;
-        y <- getRegister rs2;
-        pc <- getPC;
-        if wlt_dec x y then Return tt else (setPC (pc ^+ (signed_lit_to_word sbimm12)))
+        setRegister rd (wxor x y)
+
+    (* ``The jump and link (JAL) instruction uses the J-type format, where the J-immediate encodes
+       a signed offset in multiples of 2 bytes. The offset is sign-extended and added to the pc to
+       form the jump target address. Jumps can therefore target a +/- 1 MiB range. JAL stores the
+       address of the instruction following the jump (pc+4) into register rd.'' *)
     | Jal rd jimm20 =>
         pc <- getPC;
         setRegister rd (pc ^+ $4);;
         setPC (pc ^+ (signed_jimm_to_word jimm20))
+
+    (* ``All branch instructions use the B-type instruction format. The 12-bit B-immediate encodes
+       signed offsets in multiples of 2, and is added to the current pc to give the target address.
+       The conditional branch range is +/- 4 KiB.'' *)
+
+    (* ``BEQ and BNE take the branch if registers rs1 and rs2 are equal or unequal respectively.'' *)
+    | Beq rs1 rs2 sbimm12 =>
+        x <- getRegister rs1;
+        y <- getRegister rs2;
+        pc <- getPC;
+        if weq x y then (setPC (pc ^+ (signed_bimm_to_word sbimm12))) else Return tt
+    | Bne rs1 rs2 sbimm12 =>
+        x <- getRegister rs1;
+        y <- getRegister rs2;
+        pc <- getPC;
+        if weq x y then Return tt else (setPC (pc ^+ (signed_bimm_to_word sbimm12)))
+
+    (* ``BLT and BLTU take the branch if rs1 is less than rs2, using signed and unsigned comparison
+       respectively.'' *)
+    | Blt rs1 rs2 sbimm12 =>
+        x <- getRegister rs1;
+        y <- getRegister rs2;
+        pc <- getPC;
+        if wslt_dec x y then (setPC (pc ^+ (signed_bimm_to_word sbimm12))) else Return tt
+    | Bltu rs1 rs2 sbimm12 =>
+        x <- getRegister rs1;
+        y <- getRegister rs2;
+        pc <- getPC;
+        if wlt_dec x y then (setPC (pc ^+ (signed_bimm_to_word sbimm12))) else Return tt
+
+    (* ``BGE and BGEU take the branch if rs1 is greater than or equal to rs2, using signed and
+       unsigned comparison respectively.'' *)
+    | Bge rs1 rs2 sbimm12 =>
+        x <- getRegister rs1;
+        y <- getRegister rs2;
+        pc <- getPC;
+        if wslt_dec x y then Return tt else (setPC (pc ^+ (signed_bimm_to_word sbimm12)))
+    | Bgeu rs1 rs2 sbimm12 =>
+        x <- getRegister rs1;
+        y <- getRegister rs2;
+        pc <- getPC;
+        if wlt_dec x y then Return tt else (setPC (pc ^+ (signed_bimm_to_word sbimm12)))
+
+    (* ``MUL performs an XLEN-bit x XLEN-bit multiplication and places the lower XLEN bits in the
+       destination register.'' *)
+    | Mul rd rs1 rs2 =>
+        x <- getRegister rs1;
+        y <- getRegister rs2;
+        setRegister rd (x ^* y)
     end.
 
   Definition run1{M: Type -> Type}{MM: Monad M}{RVS: RiscvState M}: M unit :=
@@ -129,4 +253,72 @@ Section Riscv.
         rec m
     end.
   *)
+
+  Record RiscvMachine := mkRiscvMachine {
+    instructionMem: word wXLEN -> Instruction;
+    registers: Reg -> word wXLEN;
+    pc: word wXLEN;
+  }.
+
+  Instance IsRiscvMachine: RiscvState (State RiscvMachine) :=
+  {|
+      getRegister := fun (reg: Register) =>
+        match reg with
+        | RegO => Return $0
+        | RegS r => machine <- get; Return (machine.(registers) r)
+        end;
+      setRegister := fun (reg: Register) (v: word wXLEN) =>
+        match reg with
+        | RegO => Return tt
+        | RegS r => machine <- get;
+                    match machine with
+                    | mkRiscvMachine imem regs pc =>
+                        put (mkRiscvMachine imem 
+                                            (fun reg2 => if dec (r = reg2) then v else regs reg2)
+                                            pc)
+                    end
+        end;
+      loadInst := fun (addr: word wXLEN) =>
+        im <- gets instructionMem;
+        Return (im addr);
+      getPC := gets pc;
+      setPC := fun (newPC: word wXLEN) =>
+        machine <- get;
+        match machine with
+        | mkRiscvMachine imem regs pc =>
+            put (mkRiscvMachine imem regs newPC)
+        end;
+  |}.
+
+  Definition initialRiscvMachine(imem: list Instruction): RiscvMachine := {|
+    instructionMem := fun (i: word wXLEN) => nth (Nat.div (wordToNat i) 4) imem InfiniteJal;
+    registers := fun (r: Reg) => $0;
+    pc := $0
+  |}.
+
 End Riscv.
+
+
+Module MachineTest.
+
+  Definition m1: RiscvMachine 32 12 20 nat := {|
+    instructionMem := fun _ => Nop _ _ _;
+    registers := fun _ => $22;
+    pc := $33
+  |}.
+
+  Definition myInst: RiscvState 32 12 20 nat (State (RiscvMachine 32 12 20 nat)) :=
+    IsRiscvMachine _ _ _ _.
+  Existing Instance myInst.
+
+  Definition getRegister := getRegister 32 12 20 nat.
+  Definition setRegister := setRegister 32 12 20 nat.
+
+  Definition prog1: State (RiscvMachine 32 12 20 nat) (word _) :=
+    x <- getRegister (RegS _ 2);
+    setRegister (RegS _ 2) (x ^+ $3);;
+    getRegister (RegS _ 2).
+
+  Goal evalState prog1 m1 = $25. reflexivity. Qed.
+
+End MachineTest.
